theories/ITyping.v
@@ -121,6 +121,20 @@ Inductive typing (Σ : global_context) : scontext -> sterm -> sterm -> Type :=
     Σ ;;; Γ |-i p : sEq (sSort s) A B ->
     Σ ;;; Γ |-i sHeqTransport A B p t : sHeq A t B (sTransport A B p t)
 
+| type_CongProd Γ s1 s2 z1 z2 nx ny ne A1 A2 B1 B2 p q :
+    Σ ;;; Γ |-i sSort (max_sort z1 z2) : sSort (succ_sort (max_sort s1 s2)) ->
+    Σ ;;; Γ |-i A1 : sSort s1 ->
+    Σ ;;; Γ |-i A2 : sSort z1 ->
+    Σ ;;; Γ ,, svass nx A1 |-i B1 : sSort s2 ->
+    Σ ;;; Γ ,, svass ny A2 |-i B2 : sSort z2 ->
+    Σ ;;; Γ |-i p : sHeq (sSort s1) A1 (sSort z1) A2 ->
+    Σ ;;; Γ ,, svass nx A1 ,, svass ny (lift0 1 A2) ,,
+      svass ne (sHeq (lift0 2 A1) (sRel 1) (lift0 2 A2) (sRel 0)) |-i
+    q : sHeq (sSort s2) (lift0 2 B1) (sSort z2) (lift0 1 (lift 1 1 B1)) ->
+    Σ ;;; Γ |-i sCongProd A1 A2 B1 B2 p q :
+    sHeq (sSort (max_sort s1 s2)) (sProd nx A1 B1)
+         (sSort (max_sort z1 z2)) (sProd ny A2 B2)
+
 | type_conv Γ t A B s :
     Σ ;;; Γ |-i t : A ->
     Σ ;;; Γ |-i B : sSort s ->
@@ -405,6 +419,11 @@ Proof.
   - exists (succ_sort s). apply type_Heq ; assumption.
   - exists (succ_sort s). apply type_Heq. all: try assumption.
     eapply type_Transport ; eassumption.
+  - exists (succ_sort (succ_sort (max_sort s1 s2))).
+    apply type_Heq. all: try assumption.
+    + eapply type_Sort. apply (typing_wf H).
+    + apply type_Prod ; assumption.
+    + apply type_Prod ; assumption.
   - exists s. assumption.
 Defined.
 
@@ -862,3 +881,29 @@ Proof.
   destruct (inversionEq i) as [? [[[? ?] ?] ?]].
   eapply type_HeqTransport ; eassumption.
 Defined.
+
+Lemma type_CongProd' :
+  forall {Σ Γ s1 s2 z1 z2 nx ny ne A1 A2 B1 B2 p q},
+    Σ ;;; Γ,, svass nx A1 |-i B1 : sSort s2 ->
+    Σ ;;; Γ,, svass ny A2 |-i B2 : sSort z2 ->
+    Σ ;;; Γ |-i p : sHeq (sSort s1) A1 (sSort z1) A2 ->
+    Σ ;;; Γ ,, svass nx A1 ,, svass ny (lift0 1 A2) ,,
+      svass ne (sHeq (lift0 2 A1) (sRel 1) (lift0 2 A2) (sRel 0)) |-i
+    q : sHeq (sSort s2) (lift0 2 B1) (sSort z2) (lift0 1 (lift 1 1 B1)) ->
+    Σ ;;; Γ |-i sCongProd A1 A2 B1 B2 p q :
+    sHeq (sSort (max_sort s1 s2)) (sProd nx A1 B1)
+         (sSort (max_sort z1 z2)) (sProd ny A2 B2).
+Proof.
+  intros Σ Γ s1 s2 z1 z2 nx ny ne A1 A2 B1 B2 p q hB1 hB2 hp hq.
+  destruct (istype_type hp) as [? ip].
+  destruct (inversionHeq ip) as [? [[[[? ?] ?] ?] ?]].
+  destruct (istype_type hq) as [? iq].
+  destruct (inversionHeq iq) as [? [[[[? ?] ?] ?] ?]].
+  eapply type_CongProd.
+  all: try eassumption.
+  pose proof (sorts_in_sort t t0).
+  pose proof (sorts_in_sort t3 t4).
+  set (Δ := ((Γ,, svass nx A1),, svass ny (lift0 1 A2)),,
+       svass ne (sHeq (lift0 2 A1) (sRel 1) (lift0 2 A2) (sRel 0))) in H0.
+  admit.
+Admitted.
